Move [_auto_node_in_valid_dll_is_valid] and make it unpatterned

ind/DoublyLinkedListIface.fst
@@ -93,6 +93,17 @@ let dll_tail d =
   L.lemma_unsnoc_is_last (as_list h0 d);
   (!*d).DLL.ltail
 
+/// Useful auxiliary lemma
+
+(** If a node is inside a valid list, then the node is valid. *)
+val lemma_node_in_valid_dll_is_valid (h:HS.mem) (d:dll 'a) (n:node 'a) :
+  Lemma
+    (requires (dll_valid h d /\ n `L.memP` as_list h d))
+    (ensures (node_valid h n))
+let lemma_node_in_valid_dll_is_valid h d n =
+  let pos = L.index_of (as_list h d) n in
+  DLL.extract_nodelist_contained h (as_list h d) pos
+
 /// Moving forwards or backwards in a list
 
 let next_node d n =
@@ -174,15 +185,3 @@ let dll_remove_mid d n =
 /// manually. If you do, it is (likely) a bug wrt the patterns, and
 /// you should ask someone who knows about how this library works to
 /// look at things.
-
-val _auto_node_in_valid_dll_is_valid (h:HS.mem) (d:dll 'a) (n:node 'a) :
-  Lemma
-    (requires (dll_valid h d /\ n `L.memP` as_list h d))
-    (ensures (node_valid h n))
-    [SMTPat (dll_valid h d);
-     SMTPat (n `L.memP` as_list h d);
-     SMTPat (node_valid h n)]
-  // TODO: Figure out if I should really be keeping this here
-let _auto_node_in_valid_dll_is_valid h d n =
-  let pos = L.index_of (as_list h d) n in
-  DLL.extract_nodelist_contained h (as_list h d) pos
